books/projects/rp-rewriter/meta/top.lisp
@@ -46,5 +46,6 @@
 ;;(include-book "implies-meta")
 (include-book "cons-to-list-meta")
 (include-book "casesplitter")
+(include-book "casesplit-from-context")
 
 (attach-meta-fncs built-in-metas)
